basic definitions

STLC/Basic.lean
@@ -1,1 +1,246 @@
-def hello := "world"
+
+-- de-brujin syntax for the simply typed lambda calculus with numbers, bools and pairs
+
+inductive type : Type where
+  | TNat
+  | TBool
+  | Mult (τ1 τ2 : type)
+  | Arr (τ1 τ2 : type)
+
+open type
+
+@[reducible]
+def context : Type := List type
+
+inductive term : Type where
+  -- basic λ calculus terms
+  | Var (i : Nat)
+  | Abs (τ : type) (e : term)
+  | App (e1 e2 : term)
+
+  -- numbers
+  | Zro
+  | Succ (e : term)
+  | IsZero (e : term)
+
+  -- bools
+  | Fls
+  | Tru
+  | If (e1 e2 e3 : term)
+
+  -- pairs
+  | Pair (e1 e2 : term)
+  | Fst (e1 : term)
+  | Snd (e1 : term)
+
+open term
+open List
+
+inductive wt : context -> term -> type -> Prop where
+  | T_Var Γ i τ :
+    Γ[i]? = some τ ->
+    --------------------------------
+    wt Γ (Var i) τ
+
+  | T_Abs Γ τ1 τ2 e :
+    wt (τ1 :: Γ) e τ2 ->
+    --------------------------------
+    wt Γ (Abs τ1 e) (Arr τ1 τ2)
+
+  | T_App Γ τ1 τ2 e1 e2 :
+    wt Γ e1 (Arr τ1 τ2) ->
+    wt Γ e2 τ1 ->
+    --------------------------------
+    wt Γ (App e1 e2) τ2
+
+  | T_Zero Γ : wt Γ Zro TNat
+
+  | T_Succ Γ e :
+    wt Γ e TNat ->
+    --------------------------------
+    wt Γ (Succ e) TNat
+
+  | T_IsZero Γ e :
+    wt Γ e TNat ->
+    --------------------------------
+    wt Γ (IsZero e) TBool
+
+  | T_True Γ : wt Γ Tru TBool
+
+  | T_Fls Γ : wt Γ Tru TBool
+
+  | T_If Γ e1 e2 e3 τ :
+    wt Γ e1 TBool ->
+    wt Γ e2 τ ->
+    wt Γ e3 τ ->
+    --------------------------------
+    wt Γ (If e1 e2 e3) τ
+
+  | T_Pair Γ e1 e2 τ1 τ2 :
+    wt Γ e1 τ1 ->
+    wt Γ e2 τ2 ->
+    --------------------------------
+    wt Γ (Pair e1 e2) (Mult τ1 τ2)
+
+  | T_Fst Γ e1 τ1 τ2 :
+    wt Γ e1 (Mult τ1 τ2) ->
+    --------------------------------
+    wt Γ (Fst e) τ1
+
+  | T_Snd Γ e1 τ1 τ2 :
+    wt Γ e1 (Mult τ1 τ2) ->
+    --------------------------------
+    wt Γ (Snd e) τ1
+
+open wt
+
+notation Γ "⊢" e ":" τ => wt Γ e τ
+
+def up_term (e : term) (below : Nat) : term :=
+  match e with
+  | Var i => if i < below then Var i else Var (i + 1)
+  | Abs τ e => Abs τ (up_term e (below + 1) )
+  | App e1 e2 => App (up_term e1 below) (up_term e2 below)
+  | Zro => Zro
+  | Succ e => Succ (up_term e below)
+  | IsZero e => IsZero (up_term e below)
+  | Fls => Fls
+  | Tru => Tru
+  | If e1 e2 e3 => If (up_term e1 below) (up_term e2 below) (up_term e3 below)
+  | Pair e1 e2 => Pair (up_term e1 below) (up_term e2 below)
+  | Fst e => Fst (up_term e below)
+  | Snd e => Snd (up_term e below)
+
+def subst (e : term) (var : Nat) (e' : term) : term :=
+  match e with
+  | Var i => if i == var then e' else e
+  | Abs τ e => Abs τ (subst e (var + 1) (up_term e' 0) )
+  | App e1 e2 => App (subst e1 var e') (subst e2 var e')
+  | Zro => Zro
+  | Succ e => Succ (subst e var e')
+  | IsZero e => IsZero (subst e var e')
+  | Fls => Fls
+  | Tru => Tru
+  | If e1 e2 e3 => If (subst e1 var e') (subst e2 var e') (subst e3 var e')
+  | Pair e1 e2 => Pair (subst e1 var e') (subst e2 var e')
+  | Fst e => Fst (subst e var e')
+  | Snd e => Snd (subst e var e')
+
+notation e "[" e' "]" => subst e 0 e'
+
+def is_value (e : term) : Prop :=
+  match e with
+  | Zro => true
+  | Tru => true
+  | Fls => true
+  | Var _ => true
+  | Abs _ _ => true
+  | IsZero _ => false
+  | If _ _ _ => false
+  | Fst _ => false
+  | Snd _ => false
+  | App _ _ => false
+  | Succ e => is_value e
+  | Pair e1 e2 => is_value e1 /\ is_value e2
+
+inductive step : term -> term -> Prop where
+  | E_App1 e1 e1' e2 :
+      step e1 e1' ->
+    --------------------------------
+      step (App e1 e2) (App e1' e2)
+
+  | E_App2 v e2' e2 :
+    is_value v ->
+    step e2 e2' ->
+  --------------------------------
+    step (App v e2) (App v e2')
+
+  | E_AppAbs τ e v :
+    is_value v ->
+  --------------------------------
+    step (App (Abs τ e) v) (e[v])
+
+  | E_Succ e e' :
+      step e e' ->
+    --------------------------------
+      step (Succ e) (Succ e')
+
+  | E_IsZero e e' :
+      step e e' ->
+    --------------------------------
+      step (IsZero e) (IsZero e')
+
+  | E_IsZeroTrue :
+    --------------------------------
+      step (IsZero Zro) Tru
+
+  | E_IsZeroFalse v :
+      is_value v ->
+    --------------------------------
+      step (IsZero (Succ v)) Fls
+
+  | E_If e1 e1' e2 e3 :
+      step e1 e1' ->
+    --------------------------------
+      step (If e1 e2 e3) (If e1' e2 e3)
+
+  | E_IfTrue e2 e3 :
+    --------------------------------
+      step (If Tru e2 e3) e2
+
+  | E_IfFalse e2 e3 :
+    --------------------------------
+      step (If Fls e2 e3) e3
+
+  | E_Pair1 e1 e1' e2 :
+      step e1 e1' ->
+    --------------------------------
+      step (Pair e1 e2) (Pair e1' e2)
+
+  | E_Pair2 v e2' e2 :
+    is_value v ->
+    step e2 e2' ->
+  --------------------------------
+    step (Pair v e2) (Pair v e2')
+
+  | E_Fst e e' :
+      step e e' ->
+    --------------------------------
+      step (Fst e) (Fst e')
+
+  | E_FstPair v1 v2 :
+      is_value v1 ->
+      is_value v2 ->
+    --------------------------------
+      step (Fst (Pair v1 v2)) v1
+
+  | E_Snd e e' :
+      step e e' ->
+    --------------------------------
+      step (Snd e) (Snd e')
+
+  | E_SndPair v1 v2 :
+      is_value v1 ->
+      is_value v2 ->
+    --------------------------------
+      step (Snd (Pair v1 v2)) v2
+
+notation e ">->" e' => step e e'
+
+open step
+
+inductive multistep : term -> term -> Prop where
+  | M_refl e : multistep e e
+  | M_one e1 e2 e3 :
+      (e1 >-> e2) ->
+      multistep e2 e3 ->
+      multistep e1 e3
+
+notation e ">->*" e' => multistep e e'
+
+open multistep
+
+theorem normalizing : forall Γ e τ,
+  (Γ ⊢ e : τ) ->
+  exists e', (e >->* e') /\ is_value e' := by
+  sorry
